[lf] Wip on the dlm_db_example proof.

aneris/examples/reliable_communication/examples/dlm_db_example/dlm_db_example_proof.v
@@ -20,165 +20,121 @@ From aneris.examples.reliable_communication.lib.repdb.spec
 From aneris.examples.reliable_communication.examples.dlm_db_example
      Require Import dlm_db_example_code.
 
-(* -------------------------------------------------------------------------- *)
-(** The definition of the user parameters for DB and DL. *)
-(* -------------------------------------------------------------------------- *)
-Definition DBSrv (sa saF : socket_address) : DB_params :=
-  {| DB_addr := sa;
-    DB_addrF := saF;
-    DB_keys := {["x"; "y"]};
-    DB_InvName := (nroot .@ "DBInv");
-    DB_serialization := int_serialization;
-    DB_ser_inj := int_ser_is_ser_injective;
-    DB_ser_inj_alt := int_ser_is_ser_injective_alt |}.
-
-
-Definition DLSrv (sa : socket_address) : DL_params :=
-  {| DL_server_addr := sa;
-    DL_namespace := (nroot .@ "DLInv"); |}.
 
 (* -------------------------------------------------------------------------- *)
 (** The definition of the resource guarded by the distributed lock manager. *)
 (* -------------------------------------------------------------------------- *)
-Section Shared_resource_def.
-  Context `{!anerisG Mdl Σ}.
-  Context `{!DB_time, !DBG Σ}.
-  Context (DBP: DB_params).
-  Context `{!@DB_resources _ _ _ _ DBP}.
+Section proof_of_code.
+  Context `{!anerisG Mdl Σ, !lockG Σ}.
+  Context `{TM: !DB_time, !DBG Σ}.
+  Context (leader_si : message → iProp Σ).
+  Context (db_sa db_Fsa dlm_sa : socket_address).
+
+  (* ------------------------------------------------------------------------ *)
+  (** The definition of the parameters for DB and DL and shared resources. *)
+  (* ------------------------------------------------------------------------ *)
+
+  Local Instance DLSrv : DL_params :=
+    {|
+      DL_server_addr := dlm_sa;
+      DL_namespace := (nroot .@ "DLInv");
+    |}.
+
+  Local Instance DBSrv : DB_params :=
+    {|
+      DB_addr := db_sa;
+      DB_addrF := db_Fsa;
+      DB_keys := {["x"; "y"]};
+      DB_InvName := (nroot .@ "DBInv");
+      DB_serialization := int_serialization;
+      DB_ser_inj := int_ser_is_ser_injective;
+      DB_ser_inj_alt := int_ser_is_ser_injective_alt
+    |}.
+
+  Context `{!@DB_resources _ _ _ _ DBSrv}.
+  Context `{!DlockG Σ, !DL_resources}.
 
   Definition SharedRes : iProp Σ :=
-    ∃ (xv yv : option we) (h : ghst),
-      "x" ↦ₖ xv ∗
-      "y" ↦ₖ yv ∗
-      Obs DB_addr h ∗
-      ⌜at_key "x" h = xv⌝ ∗
-      ⌜at_key "y" h = yv⌝ ∗
-      ⌜∀ xw yw,
-         (xv = Some xw ∧ xw.(we_val) = #37) ↔
-         (yv = Some yw ∧ yw.(we_val) = #1)⌝.
+      ∃ (xv yv : option we) (h : ghst),
+        "x" ↦ₖ xv ∗
+        "y" ↦ₖ yv ∗
+        Obs DB_addr h ∗
+        ⌜at_key "x" h = xv⌝ ∗
+        ⌜at_key "y" h = yv⌝ ∗
+        ⌜∀ xw yw,
+           (xv = Some xw ∧ xw.(we_val) = #37) ↔
+           (yv = Some yw ∧ yw.(we_val) = #1)⌝.
 
-End Shared_resource_def.
+  (* ------------------------------------------------------------------------ *)
+  (** The proof of the internal do_writes call *)
+  (* ------------------------------------------------------------------------ *)
+  Section proof_of_the_do_writes.
+    Context (dl : val) (clt_00 : socket_address).
+    Context (wr : val) (clt_01 : socket_address).
+    Context (HWriteSpec : ⊢ ∀ k v h, simplified_write_spec wr clt_01 k v h).
+    Context (HAcqSpec : dl_acquire_spec SharedRes clt_00 dl).
+    Context (HRelSpec : dl_release_spec SharedRes clt_00 dl).
 
+    Lemma wp_do_writes :
+      ip_of_address clt_00 = ip_of_address clt_01 →
+      {{{ DLockCanAcquire clt_00 dl SharedRes }}}
+        do_writes dl wr @[ip_of_address clt_00]
+      {{{ RET #(); True }}}.
+    Proof.
+      iIntros (HipEq Φ) "Hacq HΦ".
+      rewrite /do_writes.
+      wp_pures.
+      wp_apply (HAcqSpec with "[$Hacq]").
+      iIntros (v) "(-> & Hrel & Hdlk & Hres)".
+      wp_pures.
+      iDestruct "Hres" as (xv yv h) "(Hx & Hy & #Hobs & %Hhx & %Hhy & Hcnd)".
+      rewrite HipEq.
+      wp_apply (HWriteSpec $! "x" (SerVal #37) h _ with "[Hx Hobs]").
+      { iExists _. iFrame "#∗". done. }
+      iIntros "Hpost".
+    Admitted.
 
+  End proof_of_the_do_writes.
 
-(* -------------------------------------------------------------------------- *)
-(** The proof of the internal do_writes call *)
-(* -------------------------------------------------------------------------- *)
-Section proof_of_the_do_writes.
-  (* NotaBene : Leader-Followers resources must be introduced before the
-     distributed lock resources, because the shared resource definition above
-     involves abstract memory pointers.  *)
-  Context `{!anerisG Mdl Σ, !lockG Σ}.
-  Context (sa sFa : socket_address).
-  Notation DBP := (DBSrv sa sFa).
-  (* Leader-Followers top-level resources. *)
-  Context `{TM: !DB_time, !DBG Σ}.
-  (* Context `{DBP: !DB_params}. *)
-  Context `{!@DB_resources _ _ _ _ DBP }.
-  Notation DLRes := (SharedRes DBP).
-  (* Leader-Followers allocated resources (per call of `do_writes`) *)
-  Context (wr : val) (clt_01 : socket_address).
-  Context (HWriteSpec : ⊢ ∀ k v h, simplified_write_spec wr clt_01 k v h).
-
-  (* Distributed Lock top-level resources. *)
-  Context `{!DlockG Σ, !DL_resources}.
-  (* Distributed Lock allocated resources (per call of `do_writes`) *)
-  Context (dl : val) (clt_00 : socket_address).
-  Context (HAcqSpec : dl_acquire_spec DLRes clt_00 dl).
-  Context (HRelSpec : dl_release_spec DLRes clt_00 dl).
-  Context (HipEq : ip_of_address clt_00 = ip_of_address clt_01).
-
-  Lemma wp_do_writes :
-    {{{ DLockCanAcquire clt_00 dl DLRes }}}
-      do_writes dl wr @[ip_of_address clt_00]
-    {{{ RET #(); True }}}.
-  Proof.
-    iIntros (Φ) "Hacq HΦ".
-    rewrite /do_writes.
-    wp_pures.
-    wp_apply (HAcqSpec with "[$Hacq]").
-    iIntros (v) "(-> & Hrel & Hdlk & Hres)".
-    wp_pures.
-    iDestruct "Hres" as (xv yv h) "(Hx & Hy & #Hobs & %Hhx & %Hhy & Hcnd)".
-    rewrite HipEq.
-    wp_apply (HWriteSpec $! "x" (SerVal #37) h _ with "[Hx Hobs]").
-    { iExists _. iFrame "#∗". done. }
-    iIntros "Hpost".
-  Admitted.
-
-End proof_of_the_do_writes.
-
-(* -------------------------------------------------------------------------- *)
-(** The proof of the internal do_reads call *)
-(* -------------------------------------------------------------------------- *)
-Section proof_of_the_do_reads.
-  (* NotaBene : Leader-Followers resources must be introduced before the
-     distributed lock resources, because the shared resource definition above
-     involves abstract memory pointers.  *)
-  Context `{!anerisG Mdl Σ, !lockG Σ}.
-  Context (sa sFa : socket_address).
-  Notation DBP := (DBSrv sa sFa).
-  (* Leader-Followers top-level resources. *)
-  Context `{TM: !DB_time, !DBG Σ}.
-  (* Context `{DBP: !DB_params}. *)
-  Context `{!@DB_resources _ _ _ _ DBP }.
-  Notation DLRes := (SharedRes DBP).
-  (* Leader-Followers allocated resources (per call of `do_reads`) *)
-  Context (rd : val) (clt_11 : socket_address).
-  Context (HReadSpec : ⊢ ∀ k q h, @read_spec _ _ _ _ DBP _ rd clt_11 k q h).
-   (* Distributed Lock top-level resources. *)
-  Context `{!DlockG Σ, !DL_resources}.
-  (* Distributed Lock allocated resources (per call of `do_writes`) *)
-  Context (dl : val) (clt_10 : socket_address).
-  Context (HAcqSpec : dl_acquire_spec DLRes clt_10 dl).
-  Context (HRelSpec : dl_release_spec DLRes clt_10 dl).
-  Context (HipEq : ip_of_address clt_10 = ip_of_address clt_11).
+  (* ------------------------------------------------------------------------ *)
+  (** The proof of the internal do_reads call *)
+  (* ------------------------------------------------------------------------ *)
+  Section proof_of_the_do_reads.
+    Context (dl : val) (clt_10 : socket_address).
+    Context (rd : val) (clt_11 : socket_address).
+    Context (HReadSpec : ⊢ ∀ k q h, read_spec rd clt_11 k q h).
+    Context (HAcqSpec : dl_acquire_spec SharedRes clt_10 dl).
+    Context (HRelSpec : dl_release_spec SharedRes clt_10 dl).
 
   (* NotaBene : the spec of dl_wait_on_read can be applied to
      generic key `k` and value `v` (instead of x and 37) only if
      a resource k ↦ₖ{q} v is either provided in the precondition
      or if it is also guarded by the distributed lock. *)
-  Lemma wp_dl_wait_on_read :
-    {{{ DLockCanAcquire clt_10 dl DLRes }}}
-      dl_wait_on_read dl rd #"x" #37 @[ip_of_address clt_10]
-    {{{ RET #(); True }}}.
-  Proof.
-  Admitted.
+    Lemma wp_dl_wait_on_read :
+      ip_of_address clt_10 = ip_of_address clt_11 →
+      {{{ DLockCanAcquire clt_10 dl SharedRes }}}
+        dl_wait_on_read dl rd #"x" #37 @[ip_of_address clt_10]
+      {{{ RET #(); True }}}.
+    Proof.
+    Admitted.
 
-  Lemma wp_do_reads :
-    {{{ DLockCanAcquire clt_10 dl DLRes }}}
-      do_reads dl rd @[ip_of_address clt_10]
-    {{{ RET #(); True }}}.
-  Proof.
-  Admitted.
+    Lemma wp_do_reads :
+      {{{ DLockCanAcquire clt_10 dl SharedRes }}}
+        do_reads dl rd @[ip_of_address clt_10]
+      {{{ RET #(); True }}}.
+    Proof.
+    Admitted.
 
-End proof_of_the_do_reads.
+  End proof_of_the_do_reads.
 
+  (* ------------------------------------------------------------------------ *)
+  (** The proof of the node 0 (writer) *)
+  (* ------------------------------------------------------------------------ *)
+  Section proof_of_the_node_0.
+    Context (HdbCS : ⊢ (∀ A ca, init_client_proxy_leader_spec A ca leader_si)).
+    Context (HdlCS : ⊢ (∀ sa A, dl_subscribe_client_spec SharedRes sa A)).
 
-(* -------------------------------------------------------------------------- *)
-(** The proof of the node 0 (writer) *)
-(* -------------------------------------------------------------------------- *)
-Section proof_of_the_node_0.
-  Context `{!anerisG Mdl Σ, !lockG Σ}.
-  Context (dba dbFa dlma : socket_address).
-  Notation DBP := (DBSrv dba dbFa).
-  (* Leader-Followers top-level resources. *)
-  Context `{TM: !DB_time, !DBG Σ}.
-  (* Context `{DBP: !DB_params}. *)
-  Context `{!@DB_resources _ _ _ _ DBP }.
-  Notation DLRes := (SharedRes DBP).
-  (* Distributed Lock top-level resources. *)
-  Context `{!DlockG Σ}.
-  Context (DBL := (DLSrv dlma)).
-  Context `{!DL_resources}.
-  Context (leader_si : message → iProp Σ).
-  Context (HstartProxySpec :
-            ⊢ (∀ A ca, @init_client_proxy_leader_spec _ _ _ _ DBP _ A ca leader_si)).
-  Context (HsubscribeClient :
-            ⊢ (∀ sa (A : gset socket_address),
-                 @dl_subscribe_client_spec _ _ _ DBL _ DLRes sa A)).
-
-  Lemma proof_of_node0 (clt_00 clt_01 : socket_address) (A : gset socket_address) :
+    Lemma proof_of_node0 (clt_00 clt_01 : socket_address) A :
     ip_of_address clt_00 = ip_of_address clt_01 →
     {{{
         (* preconditions for subscribing client to dlock. *)
@@ -186,71 +142,190 @@ Section proof_of_the_node_0.
         fixed A ∗
         free_ports (ip_of_address clt_00) {[port_of_address clt_00]} ∗
         clt_00 ⤳ (∅, ∅) ∗
-        dlma ⤇ dl_reserved_server_socket_interp ∗
+        dlm_sa ⤇ dl_reserved_server_socket_interp ∗
         (* preconditions to start a client proxy for the database. *)
-        ⌜dba ∈ A⌝ ∗
+        ⌜db_sa ∈ A⌝ ∗
         ⌜clt_01 ∉ A⌝ ∗
-        dba ⤇ leader_si ∗
+        db_sa ⤇ leader_si ∗
         clt_01 ⤳ (∅, ∅) ∗
         free_ports (ip_of_address clt_01) {[port_of_address clt_01]}
     }}}
-      node0 #clt_00 #clt_01 #dlma #dba @[ip_of_address clt_00]
+      node0 #clt_00 #clt_01 #dlm_sa #db_sa @[ip_of_address clt_00]
     {{{ RET #(); True }}}.
   Proof.
   Admitted.
 
-End proof_of_the_node_0.
+  End proof_of_the_node_0.
 
+  (* ------------------------------------------------------------------------ *)
+  (** The proof of the node 1 (reader) *)
+  (* ------------------------------------------------------------------------ *)
+  Section proof_of_the_node_1.
+    Context (HdbCS : ⊢ (∀ A ca, init_client_proxy_leader_spec A ca leader_si)).
+    Context (HdlCS : ⊢ (∀ sa A, dl_subscribe_client_spec SharedRes sa A)).
 
-(* -------------------------------------------------------------------------- *)
-(** The proof of the node 1 (reader) *)
-(* -------------------------------------------------------------------------- *)
-Section proof_of_the_node_1.
-  Context `{!anerisG Mdl Σ, !lockG Σ}.
-  Context (dba dbFa dlma : socket_address).
-  Notation DBP := (DBSrv dba dbFa).
-  (* Leader-Followers top-level resources. *)
-  Context `{TM: !DB_time, !DBG Σ}.
-  (* Context `{DBP: !DB_params}. *)
-  Context `{!@DB_resources _ _ _ _ DBP }.
-  Notation DLRes := (SharedRes DBP).
-  (* Distributed Lock top-level resources. *)
-  Context `{!DlockG Σ}.
-  Context (DBL := (DLSrv dlma)).
-  Context `{!DL_resources}.
-  Context (leader_si : message → iProp Σ).
-  Context (HstartProxySpec :
-            ⊢ (∀ A ca, @init_client_proxy_leader_spec _ _ _ _ DBP _ A ca leader_si)).
-  Context (HsubscribeClient :
-            ⊢ (∀ sa (A : gset socket_address),
-                 @dl_subscribe_client_spec _ _ _ DBL _ DLRes sa A)).
-
-  Lemma proof_of_node1 (clt_10 clt_11 : socket_address) (A : gset socket_address) :
-    ip_of_address clt_10 = ip_of_address clt_11 →
-    {{{
+    Lemma proof_of_node1 (clt_10 clt_11 : socket_address) A :
+      ip_of_address clt_10 = ip_of_address clt_11 →
+      {{{
         (* preconditions for subscribing client to dlock. *)
         ⌜clt_10 ∉ A⌝ ∗
         fixed A ∗
         free_ports (ip_of_address clt_10) {[port_of_address clt_10]} ∗
         clt_10 ⤳ (∅, ∅) ∗
-        dlma ⤇ dl_reserved_server_socket_interp ∗
+        dlm_sa ⤇ dl_reserved_server_socket_interp ∗
         (* preconditions to start a client proxy for the database. *)
-        ⌜dba ∈ A⌝ ∗
+        ⌜db_sa ∈ A⌝ ∗
         ⌜clt_11 ∉ A⌝ ∗
-        dba ⤇ leader_si ∗
+        db_sa ⤇ leader_si ∗
         clt_11 ⤳ (∅, ∅) ∗
         free_ports (ip_of_address clt_11) {[port_of_address clt_11]}
-    }}}
-      node0 #clt_10 #clt_11 #dlma #dba @[ip_of_address clt_10]
-    {{{ RET #(); True }}}.
+      }}}
+        node1 #clt_10 #clt_11 #dlm_sa #db_sa @[ip_of_address clt_10]
+      {{{ RET #(); True }}}.
+    Proof.
+    Admitted.
+
+  End proof_of_the_node_1.
+
+End proof_of_code.
+
+(* From aneris.examples.reliable_communication.instantiation *)
+(*      Require Import instantiation_of_init. *)
+
+
+(** Concrete parameters (addresses, ips) *)
+Definition db_sa := SocketAddressInet "0.0.0.0" 80.
+Definition db_Fsa := SocketAddressInet "0.0.0.0" 81.
+Definition dlm_sa := SocketAddressInet "0.0.0.1" 80.
+Definition clt_sa00 := SocketAddressInet "0.0.0.2" 80.
+Definition clt_sa01 := SocketAddressInet "0.0.0.2" 81.
+Definition clt_sa10 := SocketAddressInet "0.0.0.3" 80.
+Definition clt_sa11 := SocketAddressInet "0.0.0.3" 81.
+Definition A : gset socket_address := {[ db_sa; db_Fsa; dlm_sa ]}.
+Definition ips : gset string := {[ "0.0.0.0" ; "0.0.0.1"; "0.0.0.2"; "0.0.0.3" ]}.
+Global Instance DLP : DL_params :=
+    {|
+      DL_server_addr := dlm_sa;
+      DL_namespace := (nroot .@ "DLInv");
+    |}.
+
+Global Instance DBP : DB_params :=
+    {|
+      DB_addr := db_sa;
+      DB_addrF := db_Fsa;
+      DB_keys := {["x"; "y"]};
+      DB_InvName := (nroot .@ "DBInv");
+      DB_serialization := int_serialization;
+      DB_ser_inj := int_ser_is_ser_injective;
+      DB_ser_inj_alt := int_ser_is_ser_injective_alt
+    |}.
+
+Definition main : expr :=
+    Start "0.0.0.0" (init_leader (DB_serialization.(s_serializer)) #DB_addr);;
+    Start "0.0.0.1" (dlock_start_service #dlm_sa) ;;
+    Start "0.0.0.2" (node0 #clt_sa00 #clt_sa01 #dlm_sa #db_sa).
+
+Section proof_of_main.
+  Context `{!anerisG Mdl Σ}.
+  Context `{TM: !DB_time, !DBG Σ}.
+  Context (leader_si leaderF_si : message → iProp Σ).
+  Context (Init_leader : iProp Σ).
+  Context `{!DlockG Σ, !DL_resources}.
+  Context `{DBRes : !@DB_resources _ _ _ _ DBP}.
+  Notation SharedRes := (@SharedRes _ _ _ _ db_sa db_Fsa DBRes).
+  Context (HdlSrvSpec : ⊢ (∀ A, dl_server_start_service_spec SharedRes A)).
+  Context (HdlCltSpec : ⊢ (∀ sa A, dl_subscribe_client_spec SharedRes sa A)).
+  Context (HdbSrvSpec : ⊢ (∀ A, init_leader_spec A Init_leader leader_si leaderF_si)).
+  Context (HdbCltSpec : ⊢ (∀ A ca,  init_client_proxy_leader_spec A ca leader_si)).
+
+  Lemma main_spec :
+    ⊢ |={⊤}=>
+         db_sa ⤇ leader_si -∗
+         db_Fsa ⤇ leaderF_si -∗
+         dlm_sa ⤇ dl_reserved_server_socket_interp -∗
+         fixed A -∗
+         free_ip "0.0.0.0" -∗
+         free_ip "0.0.0.1" -∗
+         free_ip "0.0.0.2" -∗
+         free_ip "0.0.0.3" -∗
+         SocketAddressInet "0.0.0.0" 80 ⤳ (∅, ∅) -∗
+         SocketAddressInet "0.0.0.0" 81 ⤳ (∅, ∅) -∗
+         SocketAddressInet "0.0.0.1" 80 ⤳ (∅, ∅) -∗
+         SocketAddressInet "0.0.0.2" 80 ⤳ (∅, ∅) -∗
+         SocketAddressInet "0.0.0.2" 81 ⤳ (∅, ∅) -∗
+         SocketAddressInet "0.0.0.3" 80 ⤳ (∅, ∅) -∗
+         SocketAddressInet "0.0.0.3" 81 ⤳ (∅, ∅) -∗
+         dl_service_init -∗
+         Init_leader -∗
+         WP main @["system"]
+      {{ v, True }}.
   Proof.
   Admitted.
 
-End proof_of_the_node_1.
+End proof_of_main.
 
 (* -------------------------------------------------------------------------- *)
 (** The proof of adequacy. *)
 (* -------------------------------------------------------------------------- *)
-Section proof_of_adequacy.
-(* TODO. *)
-End proof_of_adequacy.
+
+Definition init_state :=
+  {|
+    state_heaps := {[ "system" := ∅ ]};
+    state_sockets := {[ "system" := ∅ ]};
+    state_ports_in_use :=
+      <["0.0.0.0" := ∅ ]> $
+      <["0.0.0.1" := ∅ ]> $
+      <["0.0.0.2" := ∅ ]> $
+      <["0.0.0.3" := ∅ ]> $ ∅;
+    state_ms := ∅;
+  |}.
+
+Definition fixed_dom : gset socket_address := {[ db_sa; db_Fsa; dlm_sa ]}.
+
+Definition dummy_model := model unit (fun x y => True) ().
+
+Lemma dummy_model_finitary : adequacy.aneris_model_rel_finitary dummy_model.
+Proof.
+ intros st.
+ intros f Hnot.
+ pose proof (Hnot 0%nat 1%nat) as H.
+ assert (0%nat = 1%nat -> False) as Himpl. {
+   intros Heq.
+   discriminate Heq.
+ }
+ apply Himpl; apply H.
+ destruct (f 0%nat) as [s0 r0].
+ destruct (f 1%nat) as [s1 r1].
+ destruct s0, s1, st, r0, r1.
+ reflexivity.
+Qed.
+
+From aneris.aneris_lang.program_logic Require Import aneris_adequacy.
+From aneris.examples.reliable_communication.lib.repdb
+     Require Import model.
+
+Definition socket_interp `{!anerisG empty_model Σ}
+  db_si dbF_si dlm_si sa : socket_interp Σ :=
+  (match sa with
+   | SocketAddressInet "0.0.0.0" 80 =>  db_si
+   | SocketAddressInet "0.0.0.0" 81 =>  dbF_si
+   | SocketAddressInet "0.0.0.1" 80 =>  dlm_si
+
+   | _ => λ msg, ⌜True⌝
+   end)%I.
+
+Theorem adequacy : aneris_adequate main "system" init_state (λ _, True).
+Proof.
+  set (Σ := #[anerisΣ dummy_model; DBΣ]).
+  eapply (@adequacy
+            Σ dummy_model _ _ ips fixed_dom
+            {[db_sa; db_Fsa; clt_sa00; clt_sa01; clt_sa10; clt_sa11]} ∅ ∅ ∅);
+    try done; last first.
+  { set_solver. }
+  { intros i. rewrite /ips !elem_of_union !elem_of_singleton.
+    intros [|]; subst; simpl; set_solver. }
+  { rewrite /ips /= !dom_insert_L dom_empty_L right_id_L //. set_solver. }
+  iIntros (Hdg) "".
+  2:{ apply dummy_model_finitary . }
+  admit.
+Admitted.
